progs/verif_sha.v
@@ -4,7 +4,7 @@ Require Import progs.SHA256.
 Require Import progs.sha_lemmas.
 Local Open Scope logic.
 
-Set Printing Depth 10.
+(*Set Printing Depth 10. *)
 
 Definition __builtin_read32_reversed_spec :=
  DECLARE ___builtin_read32_reversed
@@ -69,7 +69,6 @@ Definition sha256state_ (a: s256abs) (c: val) : mpred :=
 
 Definition data_block (contents: list Z) (v: val) :=
   array_at tuchar Tsh (@ZnthV tuchar (map Int.repr contents)) 0 (Zlength contents) v.
-
 
 Definition sha256_block_data_order_spec :=
   DECLARE _sha256_block_data_order
@@ -184,7 +183,15 @@ Definition Gprog : funspecs :=
   SHA256_Update_spec:: SHA256_Final_spec::
   SHA256_spec:: nil.
 
-Definition Gtot := do_builtins (prog_defs prog) ++ Gprog.
+Fixpoint do_builtins (n: nat) (defs : list (ident * globdef fundef type)) : funspecs :=
+ match n, defs with
+  | S n', (id, Gfun (External (EF_builtin _ sig) argtys resty))::defs' => 
+     (id, mk_funspec (iota_formals 1%positive argtys, resty) unit FF FF) 
+      :: do_builtins n' defs'
+  | _, _ => nil
+ end.
+
+Definition Gtot := do_builtins 3 (prog_defs prog) ++ Gprog.
 
 Lemma sha256state__isptr:
  forall a c, sha256state_ a c = !!(isptr c) && sha256state_ a c.
@@ -217,19 +224,8 @@ Definition block_data_order_loop1 :=
 Definition block_data_order_loop2 := 
    nth 1 (loops (fn_body f_sha256_block_data_order)) Sskip.
 
-(*
-Fixpoint eval_ids (ids: list ident) : environ -> list val :=
-  match ids with
-  |  id::ids' => `cons (eval_id id) (eval_ids ids')
-  | nil => `nil
- end.
-*)
-
-Lemma sha256_block_data_order_loop1_proof:
-  forall (Espec : OracleKind)
-     (b: list int) (data: val) (regs: list int),
-     length b = LBLOCK ->
-     semax (initialized _i
+Definition Delta_loop1 : tycontext :=
+ initialized _i
           (initialized _h
            (initialized _g
               (initialized _f
@@ -239,9 +235,211 @@ Lemma sha256_block_data_order_loop1_proof:
                           (initialized _b
                              (initialized _a
                                 (initialized _data
-   (func_tycontext f_sha256_block_data_order Vprog Gtot)))))))))))
+     (func_tycontext f_sha256_block_data_order Vprog Gtot)))))))))).
+
+Lemma read32_reversed_in_bytearray:
+ forall {Espec: OracleKind} Delta (ofs: int) (lo hi: Z) base e sh contents i P Q, 
+ PROPx P (LOCALx (tc_environ Delta :: Q) (SEP ())) |-- PROP ((lo <= Int.unsigned ofs <= hi-4 )%Z)
+         LOCAL (tc_expr Delta e; `(eq (offset_val ofs base)) (eval_expr e))
+         SEP () ->
+ semax Delta  (PROPx P (LOCALx Q (SEP (`(array_at tuchar sh contents lo hi base)))))
+        (Scall (Some i)
+           (Evar ___builtin_read32_reversed
+              (Tfunction (Tcons (tptr tuint) Tnil) tuint))
+           [e])
+        (normal_ret_assert
+         (PROP () 
+         (LOCALx (`(eq (Vint (big_endian_integer (fun z => contents (z+Int.unsigned ofs)%Z)))) (eval_id i)
+                        :: Q)                 
+         SEP (`(array_at tuchar sh contents lo hi base))))).
+Admitted.
+
+Lemma split_array_at:
+  forall (i : Z) (ty : type) (sh : Share.t) (contents : Z -> reptype ty)
+    (lo hi : Z) (v : val),
+  (lo <= i <= hi)%Z ->
+  array_at ty sh contents lo hi v =
+  array_at ty sh contents lo i v * array_at ty sh contents i hi v.
+Admitted.
+
+Arguments Int.unsigned n : simpl never. (*  remove this once recompiled forward.v *)
+
+Lemma semax_store_initialize_array:
+forall Espec (Delta: tycontext) n sh t1 (contents: Z -> reptype t1)
+              (lo hi: Z)
+              (v1: environ-> val) inject P Q R            
+             e1  e2 (v2: Z) (v: reptype t1),
+    writable_share sh ->
+    typeof e1 =  tptr t1 ->
+    type_is_volatile t1 = false ->
+    repinject t1 = Some inject ->
+    nth_error R n = Some (`(arrayof_' (mapsto_ Tsh t1) t1 v2 (Z.to_nat (hi-v2))) v1) ->
+    PROPx P (LOCALx (tc_environ Delta :: Q) (SEPx R)) |-- 
+          local (`eq (`(eval_binop Oadd (tptr t1) tint) v1 `(Vint (Int.repr v2))) (eval_expr e1))
+          && !! (in_range lo hi v2)
+          && local (tc_expr Delta e1) && local (tc_expr Delta (Ecast e2 t1))
+          && local (`(eq (inject v)) (eval_expr (Ecast e2 t1))) ->
+    @semax Espec Delta 
+       (|> PROPx P (LOCALx Q (SEPx R)))
+       (Sassign (Ederef e1 t1) e2) 
+       (normal_ret_assert
+          (PROPx P (LOCALx Q
+              (SEPx (replace_nth n R
+                    (`(array_at t1 sh (upd contents v2 v) lo (lo+1)) v1 *
+                     `(arrayof_' (mapsto_ Tsh t1) t1 (v2+1) (Z.to_nat (hi-(v2+1)))) v1)))))).
+Admitted.
+
+Lemma numbd_lift0:
+  forall n f,
+   numbd n (@liftx (LiftEnviron mpred) f) = 
+   (@liftx (LiftEnviron mpred)) (numbd n f).
+Proof. reflexivity. Qed.
+
+Definition rearrange_regs :=
+(Ssequence
+     (Sset _T1
+        (Ebinop Oadd
+           (Ebinop Oadd
+              (Ebinop Oadd
+                 (Ebinop Oadd (Etempvar _l tuint) (Etempvar _h tuint) tuint)
+                 (Ebinop Oxor
+                    (Ebinop Oxor
+                       (Ebinop Oor
+                          (Ebinop Oshl (Etempvar _e tuint)
+                             (Econst_int (Int.repr 26) tint) tuint)
+                          (Ebinop Oshr
+                             (Ebinop Oand (Etempvar _e tuint)
+                                (Econst_int (Int.repr (-1)) tuint) tuint)
+                             (Ebinop Osub (Econst_int (Int.repr 32) tint)
+                                (Econst_int (Int.repr 26) tint) tint) tuint)
+                          tuint)
+                       (Ebinop Oor
+                          (Ebinop Oshl (Etempvar _e tuint)
+                             (Econst_int (Int.repr 21) tint) tuint)
+                          (Ebinop Oshr
+                             (Ebinop Oand (Etempvar _e tuint)
+                                (Econst_int (Int.repr (-1)) tuint) tuint)
+                             (Ebinop Osub (Econst_int (Int.repr 32) tint)
+                                (Econst_int (Int.repr 21) tint) tint) tuint)
+                          tuint) tuint)
+                    (Ebinop Oor
+                       (Ebinop Oshl (Etempvar _e tuint)
+                          (Econst_int (Int.repr 7) tint) tuint)
+                       (Ebinop Oshr
+                          (Ebinop Oand (Etempvar _e tuint)
+                             (Econst_int (Int.repr (-1)) tuint) tuint)
+                          (Ebinop Osub (Econst_int (Int.repr 32) tint)
+                             (Econst_int (Int.repr 7) tint) tint) tuint)
+                       tuint) tuint) tuint)
+              (Ebinop Oxor
+                 (Ebinop Oand (Etempvar _e tuint) (Etempvar _f tuint) tuint)
+                 (Ebinop Oand (Eunop Onotint (Etempvar _e tuint) tuint)
+                    (Etempvar _g tuint) tuint) tuint) tuint)
+           (Etempvar _Ki tuint) tuint))
+     (Ssequence
+        (Sset _T2
+           (Ebinop Oadd
+              (Ebinop Oxor
+                 (Ebinop Oxor
+                    (Ebinop Oor
+                       (Ebinop Oshl (Etempvar _a tuint)
+                          (Econst_int (Int.repr 30) tint) tuint)
+                       (Ebinop Oshr
+                          (Ebinop Oand (Etempvar _a tuint)
+                             (Econst_int (Int.repr (-1)) tuint) tuint)
+                          (Ebinop Osub (Econst_int (Int.repr 32) tint)
+                             (Econst_int (Int.repr 30) tint) tint) tuint)
+                       tuint)
+                    (Ebinop Oor
+                       (Ebinop Oshl (Etempvar _a tuint)
+                          (Econst_int (Int.repr 19) tint) tuint)
+                       (Ebinop Oshr
+                          (Ebinop Oand (Etempvar _a tuint)
+                             (Econst_int (Int.repr (-1)) tuint) tuint)
+                          (Ebinop Osub (Econst_int (Int.repr 32) tint)
+                             (Econst_int (Int.repr 19) tint) tint) tuint)
+                       tuint) tuint)
+                 (Ebinop Oor
+                    (Ebinop Oshl (Etempvar _a tuint)
+                       (Econst_int (Int.repr 10) tint) tuint)
+                    (Ebinop Oshr
+                       (Ebinop Oand (Etempvar _a tuint)
+                          (Econst_int (Int.repr (-1)) tuint) tuint)
+                       (Ebinop Osub (Econst_int (Int.repr 32) tint)
+                          (Econst_int (Int.repr 10) tint) tint) tuint) tuint)
+                 tuint)
+              (Ebinop Oxor
+                 (Ebinop Oxor
+                    (Ebinop Oand (Etempvar _a tuint) (Etempvar _b tuint)
+                       tuint)
+                    (Ebinop Oand (Etempvar _a tuint) (Etempvar _c tuint)
+                       tuint) tuint)
+                 (Ebinop Oand (Etempvar _b tuint) (Etempvar _c tuint) tuint)
+                 tuint) tuint))
+        (Ssequence (Sset _h (Etempvar _g tuint))
+           (Ssequence (Sset _g (Etempvar _f tuint))
+              (Ssequence (Sset _f (Etempvar _e tuint))
+                 (Ssequence
+                    (Sset _e
+                       (Ebinop Oadd (Etempvar _d tuint) (Etempvar _T1 tuint)
+                          tuint))
+                    (Ssequence (Sset _d (Etempvar _c tuint))
+                       (Ssequence (Sset _c (Etempvar _b tuint))
+                          (Ssequence (Sset _b (Etempvar _a tuint))
+                             (Sset _a
+                                (Ebinop Oadd (Etempvar _T1 tuint)
+                                   (Etempvar _T2 tuint) tuint))))))))))).
+
+Lemma rearrange_regs_proof:
+ forall (Espec: OracleKind) X i (data: val) b regs
+ (Hdata: isptr data)
+ (H: length b = LBLOCK)
+ (H0: i < 16), 
+ semax (initialized _Ki (initialized _l (initialized _l' Delta_loop1)))
+  (PROP  ()
+   LOCAL 
+   (`(eq (offset_val (Int.repr (Zsucc (Z.of_nat i) * 4)) data)) (eval_id _data);
+   `(eq (Vint (big_endian_integer
+             (fun z : Z =>
+              @ZnthV tuchar (map Int.repr (intlist_to_Zlist b)) (z + Z.of_nat i * 4)))))
+       (eval_id _l);
+   `(eq X) (eval_var _X (tarray tuint 16));
+   `(eq (Vint (Int.repr (Z.of_nat i)))) (eval_id _i);
+   `(eq (map Vint (rnd_64 regs K (firstn i b))))
+     (`cons (eval_id _a)
+        (`cons (eval_id _b)
+           (`cons (eval_id _c)
+              (`cons (eval_id _d)
+                 (`cons (eval_id _e)
+                    (`cons (eval_id _f)
+                       (`cons (eval_id _g) (`cons (eval_id _h) `[])))))))))
+   SEP()) rearrange_regs
+  (normal_ret_assert
+     (PROP  (S i <= 16)
+      LOCAL  (`(eq X) (eval_var _X (tarray tuint 16));
+      `(eq (Vint (Int.repr (Z.succ (Z.of_nat i) - 1)))) (eval_id _i);
+      `(eq (offset_val (Int.repr (Z.succ (Z.of_nat i) * 4)) data)) (eval_id _data);
+      `(eq (map Vint (rnd_64 regs K (firstn (S i) b))))
+        (`cons (eval_id _a)
+           (`cons (eval_id _b)
+              (`cons (eval_id _c)
+                 (`cons (eval_id _d)
+                    (`cons (eval_id _e)
+                       (`cons (eval_id _f)
+                          (`cons (eval_id _g) (`cons (eval_id _h) `[])))))))))
+        SEP())).
+Admitted.
+
+Lemma sha256_block_data_order_loop1_proof:
+  forall (Espec : OracleKind)
+     (b: list int) (data: val) (regs: list int)
+     (Hdata: isptr data),
+     length b = LBLOCK ->
+     semax Delta_loop1
   (PROP ()
-   LOCAL (`(eq (map Vint regs)) 
+   LOCAL (`(eq (Vint (Int.repr 0))) (eval_id _i);
+               `(eq data) (eval_id _data);
+               `(eq (map Vint regs)) 
                   (`cons (eval_id _a) (`cons (eval_id _b) (`cons (eval_id _c) (`cons (eval_id _d)
                    (`cons (eval_id _e) (`cons (eval_id _f) (`cons (eval_id _g) (`cons (eval_id _h) `nil)))))
 ))))
@@ -258,12 +456,306 @@ Lemma sha256_block_data_order_loop1_proof:
 ))))
      SEP ( `(array_at tuint Tsh (@ZnthV tuint K) 0 (Zlength K))
                    (eval_expr (Evar _K256 (tarray tuint 64)));
-           `(array_at tuint Tsh (@ZnthV tuint b) 0 16) (eval_var _X (tarray tuint 16));
+           `(array_at tuint Tsh (@ZnthV tuint (map swap b)) 0 16) (eval_var _X (tarray tuint 16));
            `(data_block (intlist_to_Zlist b) data))) ).
 Proof.
-unfold block_data_order_loop1.
-intros. simpl nth.
+unfold block_data_order_loop1, Delta_loop1.
+intros.
+simpl nth; fold rearrange_regs.
+abbreviate_semax.
+name a_ _a.
+name b_ _b.
+name c_ _c.
+name d_ _d.
+name e_ _e.
+name f_ _f.
+name g_ _g.
+name h_ _h.
+name l_ _l.
+name Ki _Ki.
+name in_ _in.
+name ctx_ _ctx.
+name i_ _i.
+name data_ _data.
+assert (LBE := LBLOCK_zeq).
+normalize.
+
+Definition loop1_inv (rg0: list int) (b: list int) (data X: val) (delta: Z) (i: nat) :=
+    PROP ( i <= 16 )
+    LOCAL  (`(eq X) (eval_var _X (tarray tuint 16));
+               `(eq (Vint (Int.repr (Z.of_nat i - delta)))) (eval_id _i);
+               `(eq (offset_val (Int.repr ((Z.of_nat i)*4)) data)) (eval_id _data);
+     `(eq (map Vint (rnd_64 rg0 K (firstn i b))))
+      (`cons (eval_id _a)
+         (`cons (eval_id _b)
+            (`cons (eval_id _c)
+               (`cons (eval_id _d)
+                  (`cons (eval_id _e)
+                     (`cons (eval_id _f)
+                        (`cons (eval_id _g) (`cons (eval_id _h) `[])))))))))
+     SEP (`(array_at tuint Tsh (@ZnthV tuint K) 0 (Zlength K))
+      (eval_var _K256 (tarray tuint 64));
+    `(array_at tuint Tsh (@ZnthV tuint (map swap b)) 0 (Z.of_nat i) X);
+   `(arrayof_' (mapsto_ Tsh tuint) tuint (Z.of_nat i) (LBLOCK-i) X);
+   `(data_block (intlist_to_Zlist b) data)).
+
+apply semax_pre with (EX X:val, EX i:nat, loop1_inv regs b data X 0 i).
+unfold loop1_inv.
+go_lower.
+apply exp_right with (eval_var _X (tarray tuint 16) rho).
+apply exp_right with 0.
+(* 345,184   326,392*)
+abstract (solve [entailer!; omega]).
+(* 419,452   431,980 *)
+apply extract_exists_pre; intro X.
+
+apply semax_post' with (loop1_inv regs b data X 0 LBLOCK).
+unfold loop1_inv.
+(* 419,452  431,980 *)
+abstract 
+solve [entailer! ;
+           rewrite <- H2; repeat f_equal; 
+           symmetry; apply firstn_same; omega].
+(* 445,728  479,964 *)
+clear POSTCONDITION.
+
+apply (semax_loop _ _ (EX i:nat, loop1_inv regs b data X 1 i)).
+Focus 2. {
+apply extract_exists_pre; intro i.
+forward.
+apply exp_right with i.
+(* 452,280  481,476 *)
+abstract
+solve [unfold loop1_inv;  entailer! ; f_equal; omega].
+(* 561,900  574,392 *)
+} Unfocus.
+
+apply extract_exists_pre; intro i.
+unfold loop1_inv.
+forward_if (
+PROP  (i < 16)
+   LOCAL  (`(eq X) (eval_var _X (tarray tuint 16));
+   `(eq (Vint (Int.repr (Z.of_nat (0 + i))))) (eval_id _i);
+               `(eq (offset_val (Int.repr ((Z.of_nat i)*4)) data)) (eval_id _data);
+   `(eq (map Vint (rnd_64 regs K (firstn i b))))
+     (`cons (eval_id _a)
+        (`cons (eval_id _b)
+           (`cons (eval_id _c)
+              (`cons (eval_id _d)
+                 (`cons (eval_id _e)
+                    (`cons (eval_id _f)
+                       (`cons (eval_id _g) (`cons (eval_id _h) `[])))))))))
+   SEP 
+   (`(array_at tuint Tsh (@ZnthV tuint K) 0 (Zlength K))
+      (eval_var _K256 (tarray tuint 64));
+   `(array_at tuint Tsh (@ZnthV tuint (map swap b)) 0 (Z.of_nat i) X);
+   `(arrayof_' (mapsto_ Tsh tuint) tuint (Z.of_nat i) (LBLOCK-i) X);
+   `(data_block (intlist_to_Zlist b) data))).
+(* 587,640  592,608 *)
+abstract solve [entailer].
+(* 613,416  655,716 *)
+forward.
+(* 619,968  655,716 *)
+abstract solve [entailer; apply prop_right; clear - H2; split; [omega | f_equal; omega]].
+(* 726,056  709,784 *)
+eapply semax_pre; [ | apply semax_break ].
+unfold POSTCONDITION, abbreviate.
+unfold overridePost. rewrite if_false by congruence.
+unfold loop1_ret_assert.
+rewrite normal_ret_assert_elim.
+(* 738,188  709,784 *)
+abstract solve [entailer; 
+ assert (i=16) by omega; subst i; 
+ apply andp_right; [ apply prop_right | cancel];
+ replace 16 with LBLOCK in H3 by omega;
+ repeat split; auto].
+(* 854,860 750,176 *)
+unfold MORE_COMMANDS, POSTCONDITION, abbreviate.
+make_sequential.
+unfold loop1_ret_assert.
+apply extract_exists_post with (S i).
+rewrite inj_S.
+simpl plus.
+normalize.
+
+(* 945,760 834,556 *)
+
+do 2 apply -> seq_assoc.
+eapply semax_frame_seq
+ with (P1 := [])
+         (Q1 :=  [
+`(eq X) (eval_var _X (tarray tuint 16)),  
+`(eq (Vint (Int.repr (Z.of_nat i)))) (eval_id _i),
+`(eq (offset_val (Int.repr (Z.of_nat i * 4)) data)) (eval_id _data),
+`(eq (map Vint (rnd_64 regs K (firstn i b))))
+  (`cons (eval_id _a)
+     (`cons (eval_id _b)
+        (`cons (eval_id _c)
+           (`cons (eval_id _d)
+              (`cons (eval_id _e)
+                 (`cons (eval_id _f)
+                    (`cons (eval_id _g) (`cons (eval_id _h) `[]))))))))])
+         (Frame := [`(array_at tuint Tsh (@ZnthV tuint K) 0 (Zlength K))
+      (eval_var _K256 (tarray tuint 64)),
+   `(array_at tuint Tsh (@ZnthV tuint (map swap b)) 0 (Z.of_nat i) X),
+   `(arrayof_' (mapsto_ Tsh tuint) tuint (Z.of_nat i) (LBLOCK - i) X)]); 
+   [apply (read32_reversed_in_bytearray _ (Int.repr (Z.of_nat i * 4)) 0 (Zlength (intlist_to_Zlist b)) data _ Tsh 
+                     (@ZnthV tuchar (map Int.repr (intlist_to_Zlist b))))
+   | | | ].
+(* 945,760 834,556 *)
+abstract solve [entailer!; try omega; 
+ rewrite Zlength_correct; rewrite length_intlist_to_Zlist; rewrite H;
+ replace (Z.of_nat (4 * LBLOCK) - 4)%Z
+  with ((Z.of_nat LBLOCK - 1) * 4)%Z; 
+    [apply Zmult_le_compat_r; omega | ];
+ rewrite Zmult_comm;
+ rewrite Z.mul_sub_distr_l;
+ reflexivity].
+(* 990,216 849,172 *)
+abstract solve [entailer!].
+(* 1,078,128 849,172 *)
+auto 50 with closed.
+simpl.
+change (array_at tuchar Tsh (@ZnthV tuchar (map Int.repr (intlist_to_Zlist b))) 0
+        (Zlength (intlist_to_Zlist b)) data)
+  with (data_block  (intlist_to_Zlist b) data).
+
+forward. (* l := l'; *)
+forward. (* data := data + 4; *)
+(* 1,194,800 849,172 *)
+abstract solve [entailer!].
+(* 1,254,920 849,172 *)
+normalize.
+(* 1,291,784 894,136 *)
+simpl typeof.
+
+replace (LBLOCK-i) with (Z.to_nat (Z.of_nat LBLOCK - Z.of_nat i))
+ by (rewrite Z2Nat.inj_sub by omega; repeat rewrite Nat2Z.id; auto).
+
+eapply semax_seq'.
+ensure_normal_ret_assert;
+hoist_later_in_pre.
+
+match goal with
+| |- @semax ?Esp ?Delta (|> (PROPx ?P (LOCALx ?Q (SEPx ?R)))) 
+     (Sassign (Ederef (Ebinop Oadd ?e1 ?ei _) ?t) ?e2) _ =>
+  let n := fresh "n" in evar (n: nat); 
+  let sh := fresh "sh" in evar (sh: share);
+  let contents := fresh "contents" in evar (contents: Z -> reptype t);
+  let lo := fresh "lo" in evar (lo: Z);
+  let hi := fresh "hi" in evar (hi: Z);
+  let a := fresh "a" in evar (a: val);
+  let H := fresh in 
+  assert (H: PROPx P (LOCALx (tc_environ Delta :: Q) (SEPx (number_list O R))) 
+     |-- (`(numbd n (arrayof_' (mapsto_ sh t) t lo (Z.to_nat (hi-lo)) a))) * TT);
+  [unfold number_list, n, sh, contents, lo, hi, a; 
+  repeat rewrite @numbd_lift0; 
+  repeat rewrite @numbd_lift1; repeat rewrite @numbd_lift2;
+  solve [go_lower; repeat apply andp_left2; cancel ]
+ | clear H ];
+eapply(@semax_store_initialize_array _ Delta n sh tuint contents lo hi (`a));
+unfold number_list, n, sh, contents, lo, hi, a;
+  clear n sh contents lo hi a;
+  [solve [auto] | reflexivity | reflexivity 
+  | reflexivity
+  | autorewrite with norm; try reflexivity;
+    fail 4 "Cannot prove 6th premise of semax_store_initialize_array"
+  | ]
+end.
+name l'_ _l'.
+(* 1,371,592 965,884 *)
+solve [entailer!; [eapply eval_var_isptr; eauto | omega | omega]].
+(* 1,433,728 1,066,896 *)
+instantiate (1:= (@ZnthV tuint (map swap b))).
+unfold replace_nth; abbreviate_semax.
+(* 1,503,420 1,083,564 *)
+
+rewrite <- (array_at_ext tuint Tsh (@ZnthV tuint (map swap b))
+     (upd (@ZnthV tuint (map swap b)) (Z.of_nat i)
+              (big_endian_integer
+                 (fun z : Z =>
+                  @ZnthV tuchar (map Int.repr (intlist_to_Zlist b))
+                    (z + Z.of_nat i * 4))))).
+Focus 2.
+intros.
+unfold upd.
+if_tac; try auto.
+subst i0.
+unfold ZnthV.
+rewrite Nat2Z.id.
+symmetry; apply nth_big_endian_int; omega.
+(* 1,506,948 1,110,852 *)
+normalize.
+gather_SEP 4%Z 0%Z.
+replace_SEP 0%Z
+  (`(array_at tuint Tsh (@ZnthV tuint (map swap b))
+        0 (Z.of_nat i + 1) X)).
+apply andp_left2.
+apply andp_left2.
+go_lower.
+rewrite <- split_array_at.
+cancel.
+omega.
+(* 1,506,948 1,134,576 *)
+forward.  (* Ki=K256[i]; *)
+(* 1,689,280 1,212,872 *)
+abstract solve [entailer!; 
+  [omega | change (Zlength K) with 64%Z; omega 
+  | eapply eval_var_isptr; eauto]].
+(* 1,811,028 1,406,332 *)
+unfold POSTCONDITION, abbreviate; clear POSTCONDITION.
+
+match goal with 
+  |- semax _ (PROPx _ (LOCALx _ (SEPx ?R))) _ 
+       (normal_ret_assert (PROPx ?P (LOCALx ?Q _)))
+ => apply semax_post' with (PROPx P (LOCALx Q (SEPx R)));
+  [ | change R with (nil++R); apply semax_frame_PQR with (R2:=R)]
+end.
+apply andp_derives; auto.
+apply andp_derives; auto.
+replace (Z.succ (Z.of_nat i)) with (Z.of_nat i + 1)%Z by omega.
+go_lower0; cancel.
+apply derives_refl'; f_equal.
+rewrite Z2Nat.inj_sub by omega.
+repeat rewrite Nat2Z.id; auto.
+rewrite Z2Nat.inj_add by omega.
+repeat rewrite Nat2Z.id; auto.
+f_equal.
+change (Z.to_nat 1) with 1.
+clear; omega.
+auto 50 with closed.
+(* 1,811,028 1,429,048 *)
+eapply semax_pre; [ | apply rearrange_regs_proof; auto ].
+entailer!.
+destruct data; inv Hdata; simpl; f_equal.
+rewrite Int.add_assoc.
+f_equal.
+unfold Z.succ.
+rewrite Z.mul_add_distr_r.
+rewrite <- add_repr.
+f_equal.
+destruct (eval_id _l' rho); inv H2.
+inv H3; auto.
+Qed.
+
+Lemma datablock_local_facts:
+ forall f data,
+  data_block f data |-- !! (isptr data).
 Admitted.
+Hint Resolve datablock_local_facts : saturate_local.
+
+Lemma local_and_retval:
+ forall (i: ident) (P: val -> Prop) (R: mpred),
+    `(local (`P retval) && `R) (get_result1 i) = local (`P (eval_id i)) && `R.
+Proof.
+intros.
+extensionality rho.
+super_unfold_lift.
+unfold get_result1. simpl.
+unfold local, lift1.
+f_equal; auto.
+Qed.
+Hint Rewrite local_and_retval: norm.
 
 Lemma sha256_block_data_order_loop2_proof:
   forall (Espec : OracleKind)
@@ -321,8 +813,7 @@ Definition load8 id ofs :=
 
 Lemma sha256_block_load8:
   forall (Espec : OracleKind) 
-     (b: list int) (data: val) (r_h: list int) (r_data: list int)
-        (ctx: val)
+     (data: val) (r_h: list int) (ctx: val)
    (H5 : length r_h = 8),
      semax  
       (initialized _data
@@ -351,10 +842,12 @@ Lemma sha256_block_load8:
    SEP  (`(array_at tuint Tsh (@ZnthV tuint r_h) 0 (Zlength r_h) ctx)))).
 Proof.
 intros.
+simplify_Delta.
+unfold load8.
+abbreviate_semax.
 normalize.
 simpl.
 normalize.
-unfold load8.
 name a_ _a.
 name b_ _b.
 name c_ _c.
@@ -388,7 +881,6 @@ Definition get_h (n: Z) :=
                  (Ederef (Etempvar _ctx (tptr t_struct_SHA256state_st))
                     t_struct_SHA256state_st) _h (tarray tuint 8))
               (Econst_int (Int.repr n) tint) (tptr tuint)) tuint).
-
 
 Definition add_h (n: Z) (i: ident) :=
    Sassign
@@ -460,23 +952,6 @@ Admitted.
 Hint Extern 1 (array_at _ _ _ _ _ _ |-- arrayof_ _ _ _ _) =>
   (apply array_at_arrayof_; reflexivity) : cancel.
 
-Lemma semax_frame1:
- forall {Espec: OracleKind} Frame Delta 
-     P Q c R P1 Q1 R1 P2 Q2 R2,
-    semax Delta (PROPx P1 (LOCALx Q1 (SEPx R1))) c 
-                      (normal_ret_assert (PROPx P2 (LOCALx Q2 (SEPx R2)))) ->
-    PROPx P (LOCALx (tc_environ Delta :: Q) (SEPx R)) |-- 
-    PROPx P1 (LOCALx Q1 (SEPx (R1 ++ Frame))) ->
-    closed_wrt_modvars c (SEPx Frame) ->
-    semax Delta (PROPx P (LOCALx Q (SEPx R))) c 
-                      (normal_ret_assert (PROPx P2 (LOCALx Q2 (SEPx (R2++Frame))))).
-Proof.
-intros.
-eapply semax_pre.
-apply H0.
-apply semax_frame_PQR; auto.
-Qed.
-
 Lemma elim_globals_only:
   forall Delta g i t rho,
   tc_environ Delta rho /\ (glob_types Delta) ! i = Some g ->
@@ -515,39 +990,38 @@ change (length hashed = 16 * n)%nat in H4b.
 assert (length r_h = 8%nat) by (subst r_h; apply length_process_msg).
 (* assert (H5': Zlength r_h = 8) by (rewrite Zlength_correct; rewrite H5; reflexivity). *)
 forward. (* data = in; *)
-
-(**** BEGIN   the eight load-from-array-h[] commands.
-  Ideally, we'd just do it with these commands:
-forward; [entailer! ;  omega | ]. (* a = ctx->h[0]; *)
-forward; [entailer! ;  omega | ]. (* b = ctx->h[1]; *)
-forward; [entailer! ;  omega | ]. (* c = ctx->h[2]; *)
-forward; [entailer! ;  omega | ]. (* d = ctx->h[3]; *)
-forward; [entailer! ;  omega | ]. (* e = ctx->h[4]; *)
-forward; [entailer! ;  omega | ]. (* f = ctx->h[5]; *)
-forward; [entailer! ;  omega | ]. (* g = ctx->h[6]; *)
-forward; [entailer! ;  omega | ]. (* h = ctx->h[7]; *)
-but they use an extra gigabyte of memory and blow up Coq.
-So instead we use the Lemma sha256_block_load8,
- as follows.
-*)
-
+abbreviate_semax.
+match goal with |- semax _ (PROPx nil ?QR) _ _ =>
+ apply semax_pre0 with (PROPx [isptr data] QR)
+end.
+apply andp_right; [ | apply andp_left2; auto].
+entailer.
+normalize.
 match goal with |- semax _ _ ?c _ =>
  eapply seq_assocN with (cs := sequenceN 8 c)
 end.
 eapply semax_frame1.
 eapply sha256_block_load8 with (ctx:=ctx); eassumption.
+simplify_Delta; reflexivity.
 entailer!.
-unfold app; abbreviate_semax.
-(**** END   the eight load-from-array-h[] commands. *)
+auto 50 with closed.
+abbreviate_semax.
+simpl.
+change (lift1 (arrayof_ (mapsto_ Tsh tuint) tuint (Pos.to_nat 16)))
+  with (`(arrayof_ (mapsto_ Tsh tuint) tuint (Pos.to_nat 16))).
+change (lift1 (array_at tuint Tsh (@ZnthV tuint K) 0 (Zlength K)))
+    with (`(array_at tuint Tsh (@ZnthV tuint K) 0 (Zlength K))).
 
 forward.  (* i = 0; *)
 
 eapply semax_frame_seq.
-apply sha256_block_data_order_loop1_proof
-              with (regs:=r_h)(b:=b)(data:=data); try eassumption.
+replace Delta with Delta_loop1
+ by (simplify_Delta; reflexivity).
+simple apply (sha256_block_data_order_loop1_proof
+  _ b data r_h); auto.
 entailer!.
 auto 50 with closed.
-unfold app; abbreviate_semax.
+simpl; abbreviate_semax.
 
 eapply semax_frame_seq.
 apply sha256_block_data_order_loop2_proof
@@ -559,8 +1033,10 @@ eapply seq_assocN with (cs := add_them_back).
 
 eapply semax_frame1.
 apply (add_them_back_proof _ b r_h ctx hashed); try eassumption.
+simplify_Delta; reflexivity.
 entailer. cancel.
 auto 50 with closed.
+simpl; abbreviate_semax.
 
 forward.
 entailer.
